Prove if-true case of preservation part of EPP theorem

projection/proofs/bakery_to_endpointProofScript.sml
@@ -92,8 +92,17 @@ val compile_network_ok_project_ok = Q.store_thm("compile_network_ok_project_ok",
   \\ metis_tac []
 );
 
+val compile_network_ok_dest_sel = Q.store_thm("compile_network_ok_dest_sel",
+  `∀s c l p b q.
+    compile_network_ok s (Sel p b q c) l
+    ⇒ compile_network_ok s c l`,
+  Induct_on `l`
+  \\ rw [compile_network_gen_def,project_def]
+  \\ metis_tac []
+);
+
 val project_if_l_eq = Q.store_thm("project_if_l_eq",
-  `∀s v p q h c1 c2 l.
+  `∀v p q c1 c2.
     project_ok q (IfThen v p c1 c2)
     ∧ p ≠ q
     ∧ (∀b t c'. c1 ≠ Sel p b t c')
@@ -142,6 +151,29 @@ val compile_network_if_l_eq = Q.store_thm("compile_network_if_l_eq",
   \\ fs []
 );
 
+val split_sel_project_ok = Q.store_thm("split_sel_project_ok",
+  `!h p c b r. h <> p /\ split_sel h p c = SOME (b,r)
+   /\ project_ok h r
+   ==> project_ok h c`,
+  Induct_on `c` >> rw[project_def,split_sel_def]
+  >> metis_tac[]);
+
+val split_sel_project_ok2 = Q.store_thm("split_sel_project_ok2",
+  `!h p c b r. h <> p /\ split_sel h p c = SOME (b,r)
+   /\ project_ok h c
+   ==> project_ok h r`,
+  Induct_on `c` >> rw[project_def,split_sel_def]
+  >> metis_tac[]);
+
+val compile_network_if_l = Q.store_thm("compile_network_if_l",
+  `∀s v p c1 c2 l.
+    compile_network_ok s (IfThen v p c1 c2) l
+    ⇒ compile_network_ok s c1 l`,
+  Induct_on `l` >> rw[compile_network_gen_def,project_def]
+  >> every_case_tac >> fs[]
+  >> first_x_assum drule >> strip_tac >> fs[]
+  >> metis_tac[split_sel_project_ok]);
+
 val compile_network_if_r_eq = Q.store_thm("compile_network_if_r_eq",
   `∀s v p c1 c2 l.
     compile_network_ok s (IfThen v p c1 c2) l
@@ -186,6 +218,169 @@ val prefix_project_eq = Q.store_thm("prefix_project_eq",
   \\ rw [project_def,preSel_def,cut_sel_upto_def,projPre_def]
   \\ fs [project_def]
 );
+
+val list_trans_projpre = Q.store_thm("list_trans_projpre",
+  `!p sq c' e.
+     ~MEM p (MAP SND (preSel p c'))
+     ==>
+     list_trans (NEndpoint p sq (projPre p (preSel p c') e))
+                      (MAP (λ(b,q). LIntChoice p b q) (preSel p c'))
+                      (NEndpoint p sq e)`,
+  Induct_on `c'`
+  >> TRY(rw[preSel_def,projPre_def,list_trans_def] \\ NO_TAC)
+  >> rpt strip_tac
+  >> simp[preSel_def]
+  >> reverse IF_CASES_TAC
+  >- rw[preSel_def,projPre_def,list_trans_def]
+  >> rveq >> rename1 `NEndpoint p`
+  >> simp[list_trans_def,PULL_EXISTS,projPre_def]
+  >> qmatch_goalsub_abbrev_tac `IntChoice _ _ a1`
+  >> qexists_tac `NEndpoint p sq a1`
+  >> qunabbrev_tac `a1`
+  >> qpat_x_assum `¬ _` mp_tac
+  >> simp[preSel_def] >> strip_tac
+  >> simp[trans_int_choice]);
+
+(* TODO: move to endpointProps? *)
+val list_trans_com_choice_l = Q.store_thm("list_trans_com_choice_l",
+ `!icl ecl n1 n2 n1' n2'.
+  EVERY2 (\ic ec. ?p b q. ic = LIntChoice p b q /\ ec = LExtChoice p b q) icl ecl
+  /\ list_trans n1 icl n1' /\ list_trans n2 ecl n2'
+  ==>
+  reduction^* (NPar n1 n2) (NPar n1' n2')`,
+  simp[GSYM AND_IMP_INTRO, GSYM PULL_FORALL]
+  >> ho_match_mp_tac LIST_REL_ind >> rpt strip_tac
+  >> fs[list_trans_def]
+  >> rveq
+  >> match_mp_tac(CONJUNCT2(SPEC_ALL RTC_RULES))
+  >> imp_res_tac sender_receiver_distinct_choice
+  >> imp_res_tac trans_com_choice_l
+  >> simp[reduction_def]
+  >> asm_exists_tac >> simp[]);
+
+val list_trans_com_choice_l' = Q.store_thm("list_trans_com_choice_l'",
+ `!icl ecl n1 n2 n1' n2' n2''.
+  EVERY2 (\ic ec. ?p b q. ic = LIntChoice p b q /\ ec = LExtChoice p b q) icl ecl
+  /\ list_trans n1 icl n1' /\ list_trans n2 ecl n2'
+  /\ reduction^* n2' n2''
+  ==>
+  reduction^* (NPar n1 n2) (NPar n1' n2'')`,
+  metis_tac[reduction_par_r,RTC_RTC,list_trans_com_choice_l]);
+
+val trans_fold_par = Q.store_thm("trans_fold_par",
+  `!n1 e1 e2 n2 alpha. trans e1 alpha e2
+   ==> trans (FOLDR NPar NNil (n1 ++ e1::n2)) alpha (FOLDR NPar NNil (n1 ++ e2::n2))`,
+  Induct >> rw[] >> metis_tac[trans_par_l,trans_par_r]);
+
+val trans_fold_par' = Q.store_thm("trans_fold_par'",
+  `!n1 n1' e1 e2 n2 n2' alpha. trans e1 alpha e2 /\ n1 = n1' /\ n2 = n2'
+   ==> trans (FOLDR NPar NNil (n1 ++ e1::n2)) alpha (FOLDR NPar NNil (n1' ++ e2::n2'))`,
+  metis_tac[trans_fold_par]);
+
+val preSel_to_queue_def = Define
+  `preSel_to_queue proc1 proc2 l =
+    MAP (λ(b,p). (proc2,if b then [1w] else [0w])) (FILTER ($= proc1 o SND) l)`
+
+val compile_network_ok_if_eq = Q.store_thm("compile_network_ok_if_eq",
+  `!s v p c' c2 l.
+   compile_network_ok s (IfThen v p c' c2) l /\
+   ~MEM p l ==>
+   compile_network s (IfThen v p c' c2) l =
+   FOLDR NPar NNil
+   (MAP (\proc. NEndpoint proc (<| bindings := projectS proc s;
+                                   queue    := [] |>) (project' proc (IfThen v p c' c2))) l)`,
+   Induct_on `l`
+   >- rw[compile_network_gen_def]
+   >> rpt strip_tac
+   >> fs[compile_network_gen_def]
+   >> fs[project_def]);
+
+val cut_ext_choice_upto_presel_def = Define `
+   (cut_ext_choice_upto_presel p1 p2 presel Nil = Nil)
+/\ (cut_ext_choice_upto_presel p1 p2 presel (Send p v e) = Send p v e)
+/\ (cut_ext_choice_upto_presel p1 p2 presel (Receive p v e) = Receive p v e)
+/\ (cut_ext_choice_upto_presel p1 p2 presel (IfThen b e1 e2) = IfThen b e1 e2)
+/\ (cut_ext_choice_upto_presel p1 p2 presel (IntChoice p b' e) = IntChoice p b' e)
+/\ (cut_ext_choice_upto_presel p1 p2 presel (Let s f l c) = Let s f l c)
+/\ (cut_ext_choice_upto_presel p1 p2 presel (ExtChoice p e1 e2) =
+    (if p = p1 then
+      (case SPLITP ($= p2 o SND) presel of
+       (_,[]) => ExtChoice p e1 e2
+     | (_,(T,_)::presel) => cut_ext_choice_upto_presel p1 p2 presel e1
+     | (_,(F,_)::presel) => cut_ext_choice_upto_presel p1 p2 presel e2)
+     else ExtChoice p e1 e2))`
+
+val cut_ext_choice_upto_presel_nil = Q.store_thm("cut_ext_choice_upto_presel_nil",
+  `cut_ext_choice_upto_presel p1 p2 [] c = c`,
+  Induct_on `c` >> rw[cut_ext_choice_upto_presel_def,SPLITP]
+                                                );
+
+val cut_ext_choice_upto_presel_cons = Q.store_thm("cut_ext_choice_upto_presel_cons",
+  `p2 <> p3
+   ==>
+   cut_ext_choice_upto_presel p1 p2 ((b,p3)::l) c =
+   cut_ext_choice_upto_presel p1 p2 l c`,
+  Induct_on `c` >> rw[cut_ext_choice_upto_presel_def,SPLITP]
+  >> rpt(PURE_FULL_CASE_TAC >> fs[] >> rveq));
+
+val project_cut_sel_eq = Q.store_thm("project_cut_sel_eq",
+  `!h p c1.
+   p ≠ h /\ project_ok h c1 ==>
+   project' h (cut_sel_upto p c1) =
+   cut_ext_choice_upto_presel p h (preSel p c1) (project' h c1)`,
+  Induct_on `c1`
+  >- rw[cut_sel_upto_def,cut_ext_choice_upto_presel_nil,preSel_def]
+  >- rw[cut_sel_upto_def,cut_ext_choice_upto_presel_nil,preSel_def]
+  >- rw[cut_sel_upto_def,cut_ext_choice_upto_presel_nil,preSel_def]
+  >- rw[cut_sel_upto_def,cut_ext_choice_upto_presel_nil,preSel_def]
+  >> rw[cut_sel_upto_def]
+  >> simp[preSel_def] >> rw[cut_ext_choice_upto_presel_def,cut_ext_choice_upto_presel_nil]
+  >> rw[project_def,cut_ext_choice_upto_presel_def,SPLITP]
+  >> simp[cut_ext_choice_upto_presel_cons]
+  >> first_x_assum match_mp_tac >> fs[project_def] >> every_case_tac >> fs[]);
+
+val FILTER_nub = Q.store_thm("FILTER_nub",
+  `!P l. FILTER P (nub' l) = nub' (FILTER P l)`,
+  Induct_on `l` >> rpt strip_tac
+  >> fs[nub'_def] >> rw[nub'_def]
+  >> first_assum(qspec_then `P`  (assume_tac o GSYM))
+  >> first_x_assum(qspec_then `(λy. h ≠ y)` (assume_tac o GSYM))
+  >> simp[FILTER_FILTER] >> simp[Once CONJ_SYM]
+  >> rw[FILTER_EQ,EQ_IMP_THM] >> CCONTR_TAC >> fs[]);
+
+val set_nub' = Q.store_thm("set_nub'",
+  `!l. set(nub' l) = set l`,
+  Induct >> rw[nub'_def] >> simp[GSYM FILTER_nub]
+  >> simp[LIST_TO_SET_FILTER,INTER_DEF]
+  >> rw[FUN_EQ_THM,EQ_IMP_THM] >> simp[]
+  >> metis_tac[]);
+
+val compile_network_cut_sel_upto = Q.store_thm("compile_network_cut_sel_upto",
+  `!s v p c1 l.
+  compile_network_ok s c1 l /\
+  ~MEM p l ==>
+  compile_network s (cut_sel_upto p c1) l =
+  FOLDR NPar NNil
+   (MAP (\proc. NEndpoint proc (<| bindings := projectS proc s;
+                                   queue    := [] |>) (cut_ext_choice_upto_presel p proc (preSel p c1) (project' proc c1))) l)`,
+  Induct_on `l`
+  >- (rw[compile_network_gen_def])
+  >> rpt strip_tac
+  >> fs[compile_network_gen_def,project_def,
+        split_sel_def,cut_sel_upto_def,cut_ext_choice_upto_presel_def]
+  >> fs[project_cut_sel_eq]);
+
+val MEM_presel_MEM_procsOf = Q.store_thm("MEM_presel_MEM_procsOf",
+  `!c p. project_ok p c  /\ MEM p (MAP SND (preSel p c))
+   ==> F`,
+  Induct
+  >- rw[preSel_def,project_def]
+  >- rw[preSel_def,project_def]
+  >- rw[preSel_def,project_def]
+  >- rw[preSel_def,project_def]
+  >> rpt strip_tac
+  >> fs[project_def,preSel_def]
+  >> rpt(PURE_FULL_CASE_TAC >> fs[]) >> metis_tac[]);
 
 val compile_network_preservation = Q.store_thm("compile_network_preservation",
   `∀s c α τ s' c'. compile_network_ok s c (procsOf c)
@@ -350,6 +545,227 @@ val compile_network_preservation = Q.store_thm("compile_network_preservation",
      >- (Induct_on `vl` \\ rw [lookup_projectS'])
      >- (rw [projectS_fupdate] >> rpt AP_TERM_TAC
         \\ Induct_on `vl` >> rw [lookup_projectS']))
+  (* If true *)
+  >- (MAP_EVERY Q.EXISTS_TAC [`s`,`cut_sel_upto p c'`]
+     \\ rw []
+     >- (pop_assum (K ALL_TAC) >> pop_assum (K ALL_TAC)
+        \\ Induct_on `c'` >> rw [trans_s_def,cut_sel_upto_def]
+        \\ Cases_on `l0 = l` >> fs [project_def]
+        \\ ho_match_mp_tac RTC_TRANS
+        \\  metis_tac [trans_s_def,trans_sel])
+     \\ MAP_EVERY Q.ABBREV_TAC [ `l = FILTER (λy. p ≠ y) (nub' (procsOf c' ⧺ procsOf c2))`
+                               , `sq = <|bindings := projectS p s; queue := []|>`
+                               ]
+     \\ ho_match_mp_tac RTC_TRANS
+     \\ Q.EXISTS_TAC `NPar (NEndpoint p sq (SND (project p c')))
+                           (compile_network s (IfThen v p c' c2) l)`
+     \\ rw [reduction_def]
+     >- (ho_match_mp_tac trans_par_l
+        \\ ho_match_mp_tac endpointSemanticsTheory.trans_if_true
+        \\ rw [Abbr `sq`,lookup_projectS])
+     \\ `¬MEM p l` by rw [Abbr `l`,MEM_FILTER]
+     \\ rw [prefix_project_eq]
+     \\ match_mp_tac list_trans_com_choice_l'
+     \\ Q.ISPECL_THEN [`p`,`sq`,`c'`,`project' p (cut_sel_upto p c')`]
+                    mp_tac list_trans_projpre
+     \\ impl_tac
+     >- (CCONTR_TAC >> fs[] >> imp_res_tac MEM_presel_MEM_procsOf)
+     \\ strip_tac
+     \\ MAP_EVERY qexists_tac
+                  [`(MAP (λ(b,q). LIntChoice p b q) (preSel p c'))`,
+                   `(MAP (λ(b,q). LExtChoice p b q) (preSel p c'))`]
+     \\ simp[GSYM PULL_EXISTS]
+     \\ conj_tac
+     >- (simp[EVERY2_MAP,ELIM_UNCURRY]
+         \\ match_mp_tac EVERY2_refl \\ Cases \\ rw[])
+     \\ simp[compile_network_ok_if_eq]
+     \\ qexists_tac
+          `FOLDR NPar NNil
+            (MAP
+               (λproc.
+                    NEndpoint proc
+                      <|bindings := projectS proc s;
+                        queue := preSel_to_queue proc p (preSel p c')|>
+                      (project' proc (IfThen v p c' c2))) l)`
+     \\ imp_res_tac compile_network_if_l
+     \\ simp[compile_network_cut_sel_upto]
+     \\ `ALL_DISTINCT l`
+          by(qunabbrev_tac `l`
+             \\ match_mp_tac FILTER_ALL_DISTINCT
+             \\ MATCH_ACCEPT_TAC all_distinct_nub')
+     \\ `~MEM p (MAP SND (preSel p c'))`
+          by(qhdtm_x_assum `list_trans` mp_tac
+             \\ qmatch_goalsub_abbrev_tac `list_trans n1 _ n2`
+             \\ rpt(pop_assum kall_tac)
+             \\ MAP_EVERY (W(curry Q.SPEC_TAC)) [`p`,`n1`,`n2`,`c'`]
+             \\ Induct \\ rw[preSel_def,list_trans_def]
+             \\ imp_res_tac sender_receiver_distinct_choice
+             \\ metis_tac[])
+     \\ `!x. MEM x (MAP SND(preSel p c')) ==> MEM x l`
+          by(qpat_x_assum `¬_` mp_tac \\ qpat_x_assum `¬_` mp_tac
+             \\ unabbrev_all_tac \\ rpt(pop_assum kall_tac)
+             \\ simp[PULL_FORALL] \\ strip_tac \\ Induct_on `c'`
+             \\ rw[preSel_def]
+             \\ rw[procsOf_def,nub'_def]
+             \\ rw[FILTER_FILTER,FILTER_APPEND_DISTRIB]
+             \\ fs[set_nub',MEM_FILTER,MEM_MAP,PULL_EXISTS]
+             \\ rveq \\ fs[]
+             \\ fs[]
+             \\ metis_tac[])
+     \\ conj_tac
+     >- (`?qf. !proc. (qf:datum ->(datum,datum) alist) proc = []` by(qexists_tac `K []` \\ rw[])
+         \\ `!proc qff. <|bindings := projectS proc s; queue := qff proc|>
+                       = <|bindings := projectS proc s; queue := qf proc ++ qff proc|>`
+             by(rw[])
+         \\ pop_assum mp_tac \\ pop_assum kall_tac
+         \\ disch_then (fn thm => Ho_Rewrite.PURE_ONCE_REWRITE_TAC [thm])
+         \\ simp[]
+         \\ pop_assum mp_tac
+         \\ qhdtm_x_assum `ALL_DISTINCT` mp_tac
+         \\ rpt(qpat_x_assum `¬_` mp_tac) \\ rpt(pop_assum kall_tac)
+         \\ rename1 `MAP SND psl`
+         \\ MAP_EVERY (W(curry Q.SPEC_TAC))
+                      [`p`,`l`,`v`,`p`,`c'`,`c2`,`s`,`qf`,`psl`]
+         \\ Induct
+         >- (rw[list_trans_def,preSel_to_queue_def])
+         \\ rw[list_trans_def]
+         \\ rw[preSel_to_queue_def]
+         \\ `MEM (SND h) l` by simp[]
+         \\ Cases_on `h` >> simp[]
+         \\ rename1 `LExtChoice p1 b p2`
+         \\ qexists_tac
+              `FOLDR NPar NNil
+                     (MAP
+                       (λproc.
+                         NEndpoint proc
+                           <|bindings := projectS proc s; queue :=
+                             qf proc ++ if proc = p2 then [(p1, if b then [1w] else [0w])] else [] |>
+                           (project' proc (IfThen v p1 c' c2))) l)`
+         \\ conj_tac
+         >- (pop_assum(strip_assume_tac o REWRITE_RULE [MEM_SPLIT])
+             \\ simp[] \\ match_mp_tac trans_fold_par'
+             \\ conj_tac
+             >- (match_mp_tac trans_enqueue_choice_gen >> fs[])
+             \\ fs[]
+             \\ rw[MAP_EQ_f]
+             \\ rw[] \\ fs[ALL_DISTINCT_APPEND] \\ metis_tac[])
+         \\ fs[]
+         \\ first_x_assum(qspec_then `\proc. qf proc ⧺
+                          if proc = p2 then [(p1,if b then [1w] else [0w])] else []` mp_tac)
+         \\ disch_then(mp_tac o CONV_RULE(RESORT_FORALL_CONV List.rev))
+         \\ disch_then(qspecl_then [`p1`,`l`] mp_tac)
+         \\ rpt(disch_then drule)
+         \\ Ho_Rewrite.PURE_REWRITE_TAC [GSYM PULL_FORALL]
+         \\ impl_tac >- rw[]
+         \\ disch_then(qspecl_then [`v`,`c'`,`c2`,`s`] mp_tac)
+         \\ qmatch_goalsub_abbrev_tac `list_trans (FOLDR _ _ a1) _ (FOLDR _ _ a2)
+                                        ==> list_trans (FOLDR _ _ a3) _ (FOLDR _ _ a4)`
+         \\ `a1 = a3 /\ a2 = a4` suffices_by simp[]
+         \\ unabbrev_all_tac
+         \\ rw[MAP_EQ_f] \\ rw[preSel_to_queue_def])
+     \\ `?pn. pn = LENGTH(preSel p c')` by simp[]
+     \\ `!proc. MEM proc l ==> project_ok proc (if K T proc then IfThen v p c' c2 else c')`
+        by(rw[] >> imp_res_tac compile_network_ok_project_ok)
+     \\ ntac 5 (pop_assum mp_tac)
+     \\ qpat_x_assum `compile_network_ok _ (IfThen _ _ _ _) _` kall_tac
+     \\ qhdtm_x_assum `list_trans` kall_tac
+     \\ rpt(qhdtm_x_assum `Abbrev` kall_tac)
+     \\ rpt(pop_assum mp_tac)
+     \\ `!proc. project' proc (IfThen v p c' c2) = project' proc (if K T proc then IfThen v p c' c2 else c')`
+        by(rw[])
+     \\ qabbrev_tac `iffy = (K T):datum -> bool`
+     \\ pop_assum kall_tac
+     \\ pop_assum (fn thm => Ho_Rewrite.PURE_ONCE_REWRITE_TAC [thm])
+     \\ MAP_EVERY (W(curry Q.SPEC_TAC)) [`s`,`v`,`p`,`c2`,`l`,`c'`,`iffy`,`pn`]
+     \\ Induct
+     >- (rw[preSel_def,list_trans_def,cut_ext_choice_upto_presel_nil,preSel_to_queue_def]
+         >> qmatch_goalsub_abbrev_tac `_ (FOLDR NPar NNil a1) (FOLDR NPar NNil a2)`
+         >> `a1 = a2` suffices_by simp[]
+         >> unabbrev_all_tac
+         >> rw[MAP_EQ_f] >> rw[]
+         >> match_mp_tac project_if_l_eq
+         >> conj_tac
+         >- (first_x_assum drule >> fs[])
+         >> conj_tac
+         >- (CCONTR_TAC >> fs[])
+         >> CCONTR_TAC
+         >> fs[] >> rveq >> fs[preSel_def])
+     \\ rpt strip_tac
+     \\ `?b q c''. c' = Sel p b q c''`
+        by(qpat_x_assum `SUC _ = LENGTH _` mp_tac >> Cases_on `c'` >> rw[preSel_def])
+     \\ rveq
+     \\ `MEM q l` by(fs[preSel_def])
+     \\ first_assum(strip_assume_tac o REWRITE_RULE[MEM_SPLIT])
+     \\ `p <> q` by(CCONTR_TAC >> fs[])
+     \\ `project_ok q c''`
+        by(imp_res_tac compile_network_ok_project_ok
+           \\ rfs[project_def,split_sel_def]
+           \\ Cases_on `b` \\ fs[])
+     \\ first_assum drule
+     \\ strip_tac
+     \\ qmatch_goalsub_abbrev_tac `reduction^* (FOLDR NPar NNil (MAP af _))`
+     \\ qabbrev_tac `ag = \q. (NEndpoint q <|bindings := projectS q s;
+                              queue := preSel_to_queue q p (preSel p c'')|> (project' q c''))`
+     \\ `trans (af q) (LTau) (ag q)`
+        by(unabbrev_all_tac >> Cases_on `iffy q`
+           >> fs[project_def,cut_ext_choice_upto_presel_def,preSel_def,
+                 split_sel_def,compile_network_gen_def,preSel_to_queue_def]
+           >> rfs[]
+           >> rpt(PURE_CASE_TAC \\ fs[] \\ rveq)
+           >> simp[cut_ext_choice_upto_presel_def,SPLITP]
+           >> TRY(match_mp_tac trans_ext_choice_l_gen
+                  >> fs[] >> qexists_tac `[]` >> fs[])
+           >> TRY(match_mp_tac trans_ext_choice_r_gen
+                  >> fs[] >> qexists_tac `[0w]` >> qexists_tac `[]` >> fs[]))
+     \\ `trans (FOLDR NPar NNil ((MAP af l1) ++ af q :: (MAP af l2)))
+               LTau (FOLDR NPar NNil ((MAP af l1) ++ ag q :: (MAP af l2)))`
+          by(simp[trans_fold_par])
+     \\ qabbrev_tac `iffy' = λp. if p = q then F else iffy p`
+     \\ qabbrev_tac `ah = (λproc.
+                 NEndpoint proc
+                   <|bindings := projectS proc s;
+                   queue := preSel_to_queue proc p (preSel p c'')|>
+                   (project' proc (if iffy' proc then IfThen v p c'' c2 else c'')))`
+     \\ match_mp_tac(CONJUNCT2(SPEC_ALL RTC_RULES))
+     \\ qexists_tac `FOLDR NPar NNil (MAP ah l)`
+     \\ conj_tac
+     >- (simp[reduction_def]
+         \\ `MAP af l1 = MAP ah l1 /\ ag q = ah q /\ MAP af l2 = MAP ah l2`
+             suffices_by metis_tac[]
+         \\ unabbrev_all_tac
+         \\ rw[MAP_EQ_f]
+         \\ fs[preSel_def,preSel_to_queue_def,ALL_DISTINCT_APPEND]
+         \\ rpt(qpat_x_assum `trans _ _ _` kall_tac)
+         \\ `proc <> p` by(CCONTR_TAC >> fs[])
+         \\ `proc <> q` by(CCONTR_TAC >> fs[] >> metis_tac[])
+         \\ rw[] \\ fs[project_def,split_sel_def])
+     \\ first_x_assum (qspecl_then [`iffy'`,`c''`,`l`,`c2`,`p`,`v`,`s`] mp_tac)
+     \\ `project_ok p c''` by(fs[project_def])
+     \\ `compile_network_ok s c'' l` by(imp_res_tac compile_network_ok_dest_sel)
+     \\ rpt(disch_then drule)
+     \\ impl_tac
+     >- (qpat_x_assum `_ = _ ++ _::_` kall_tac
+         >> fs[preSel_def] >> unabbrev_all_tac >> fs[]
+         >> rw[] >> rpt(first_x_assum drule) >> simp[]
+         >> `proc <> p` by(CCONTR_TAC >> fs[])
+         >> fs[project_def,split_sel_def]
+         >> rw[])
+     \\ qmatch_goalsub_abbrev_tac
+          `reduction^* (FOLDR _ _ a1) (FOLDR _ _ a2) ==> reduction^* (FOLDR _ _ a3) (FOLDR _ _ a4)`
+     \\ `a1 = a3 /\ a2 = a4` suffices_by metis_tac[]
+     \\ unabbrev_all_tac
+     \\ rw[MAP_EQ_f,cut_ext_choice_upto_presel_def,preSel_def]
+     \\ `proc <> p` by(CCONTR_TAC >> fs[])
+     >- (`proc <> q` by(CCONTR_TAC >> fs[ALL_DISTINCT_APPEND] >> metis_tac[])
+         \\ fs[project_def,cut_ext_choice_upto_presel_def,cut_ext_choice_upto_presel_cons])
+     >- (fs[project_def,cut_ext_choice_upto_presel_def,cut_ext_choice_upto_presel_cons]
+         >> rw[cut_ext_choice_upto_presel_def,SPLITP])
+     >- (`proc <> q` by(CCONTR_TAC >> fs[ALL_DISTINCT_APPEND] >> metis_tac[])
+         \\ fs[project_def,cut_ext_choice_upto_presel_def,cut_ext_choice_upto_presel_cons]))
+
+  (* If false *)
+  >- cheat (* TODO *)
+
   \\ cheat
 );
 
